src/study/Nemonuri.Study.CSharpSyntaxRewriter2.Modifier/Nemonuri.StratifiedNode.Program1.fst
@@ -1,0 +1,16 @@
+module Nemonuri.StratifiedNode.Program1
+
+module L = FStar.List.Tot
+open Nemonuri.StratifiedNode
+open Nemonuri.StratifiedNode.NodeTheory
+open Nemonuri.StratifiedNode.ListTheory
+open Nemonuri.StratifiedNode.IndexTheory
+module T = Nemonuri.StratifiedNode.TypeTheory1
+
+
+let rec run (#lv:pos) (sn:T.node lv{ T.has_kind_compilation_unit sn })
+  : Tot (stratified_node_with_level T.data)
+        (decreases %[T.get_count_of_argument_need_to_substitute_expression sn])
+  = match (try_get_indexes_of_descendant_or_self_from_predicate sn T.may_have_kind_argument_need_to_substitute_expression) with
+    | None -> (assert (T.get_count_of_argument_need_to_substitute_expression sn = 0); (get_stratified_node_with_level sn))
+    | Some indexes1 -> (assert (T.get_count_of_argument_need_to_substitute_expression sn > 0); (get_stratified_node_with_level sn))
